## 26.09.2025, матанализ, 2 пара

1.

$$
1\cdot1!+2\cdot2!+3\cdot3!+\ldots+n \cdot n! = (n+1)!-1, \quad n \geq 1
$$

$$
\begin{aligned}
&\begin{array}{ll}
n=1, \quad & 1\cdot1!=2!-1 \Rightarrow 1=1; \\
n=k, \quad & 1\cdot1!+2\cdot2!+3\cdot3!+\ldots+k \cdot k! = (k+1)!-1; \\
n=k+1, \quad & 1\cdot1!+2\cdot2!+3\cdot3!+\ldots+k \cdot k! + (k+1)\cdot(k+1)! = (k+2)!-1 \\
&\end{array} \\
&(k+1)!-1+(k+1)\cdot(k+1)!=(k+2)!-1 \\
&(k+1)!\cdot(k+2)-1=(k+2)!-1 \\
&(k+2)!-1=(k+2)!-1
\end{aligned}
$$

2.

$$
\frac{1\cdot2!}{2}+\frac{2\cdot3!}{2}+\ldots+\frac{n\cdot(n+1)!}{2^n}=\frac{(n+2)!}{2^n}-2, \quad n \geq 1
$$

$$
\begin{aligned}
&\begin{array}{ll}
n=1, \quad & \frac{1\cdot2!}{2}=\frac{3!}{2}-2 \Rightarrow 1=1; \\
n=k, \quad & \frac{1\cdot2!}{2}=\frac{2\cdot3!}{2^2}+\ldots+\frac{k\cdot(k+1)!}{2^k}=\frac{(k+2)!}{2^k}-2; \\
n=k+1, \quad & \frac{1\cdot2!}{2}=\frac{2\cdot3!}{2^2}+\ldots+\frac{k\cdot(k+1)!}{2^k}+\frac{(k+1)(k+2)!}{2^{k+1}}=\frac{(k+3)!}{2^{k+1}}-2 \\
&\end{array} \\
&\frac{(k+2)!}{2^k}-2+\frac{(k+1)(k+2)!}{2^{k+1}}=\frac{(k+3)!}{2^{k+1}}-2 \\
&\frac{2\cdot(k+2)!}{2^{k+1}}-2+\frac{(k+1)(k+2)!}{2^{k+1}}=\frac{(k+3)!}{2^{k+1}}-2 \\
&\frac{(k+2)!\cdot(k+3)}{2^{k+1}}-2=\frac{(k+3)!}{2^{k+1}}-2 \\
&\frac{(k+3)!}{2^{k+1}}-2=\frac{(k+3)!}{2^{k+1}}-2
\end{aligned}
$$
