## 26.09.2025, 1 пара

1.

$$
\sum_{k=1}^{n} \frac{1}{\left(4k-3\right)\left(4k+1\right)}
$$

$$
\begin{aligned}
&\frac{1}{\left(4k-3\right)\left(4k+1\right)} = \frac{A}{4k-3}+\frac{B}{4k+1} = \frac{A\left(4k+1\right)+B\left(4k-3\right)}{\left(4k-3\right)\left(4k+1\right)} \\
&\\
&\\
&\\
&1=A\left(4k+1\right)+B\left(4k-3\right)=4Ak+A+4Bk-3B \quad \forall \space k \\
&\\
&\\
&\\
&\begin{cases}
0 = 4Ak+4Bk \Rightarrow B=-A \\
1 = A-3B
\end{cases}
\quad\Rightarrow A=\frac{1}{4}, \space B=-\frac{1}{4} \\
&\\
&\\
&\\
&\sum_{k=1}^{n} \frac{1}{\left(4k-3\right)\left(4k+1\right)} = \sum_{k=1}^{n} \frac{1/4}{4k-3}-\frac{1/4}{4k+1} \\
&= \left(\frac{1/4}{1}-\frac{1/4}{5}\right)+\left(\frac{1/4}{5}-\frac{1/4}{9}\right)+\ldots+\left(\frac{1/4}{4k-3}-\frac{1/4}{4k+1}\right) \\
&= \frac{1}{4}-\frac{1}{4\left(4k+1\right)}
\end{aligned}
$$

2.

$$
\sum_{k=1}^{n} \frac{1}{k\left(k+1\right)\left(k+2\right)}
$$

$$
\begin{aligned}
&\frac{1}{k\left(k+1\right)\left(k+2\right)} = \frac{A}{k}+\frac{B}{k+1}+\frac{C}{k+2} = \frac{A\left(k+1\right)\left(k+2\right)+Bk\left(k+2\right)+Ck\left(k+1\right)}{k\left(k+1\right)\left(k+2\right)} \\
&\\
&\\
&\\
&1=A\left(k+1\right)\left(k+2\right)+Bk\left(k+2\right)+Ck\left(k+1\right)=Ak^2+3Ak+2A+Bk^2+2Bk+Ck^2+Ck \quad \forall \space k \\
&\\
&\\
&\\
&\begin{cases}
0 = Ak^2+3Ak+Bk^2+2Bk+Ck^2+Ck \Rightarrow B=-2A, \space C=A \\
1 = 2A
\end{cases}
\quad\Rightarrow A=\frac{1}{2}, \space B=-1, \space C=\frac{1}{2}
\end{aligned}
$$

$$
\begin{aligned}
&\sum_{k=1}^{n} \frac{1}{k\left(k+1\right)\left(k+2\right)} = \sum_{k=1}^{n} \frac{1/2}{k}-\frac{1}{k+1}+\frac{1/2}{k+2} \\
&=\left(\frac{1/2}{1}-\frac{1}{2}+\frac{1/2}{3}\right)+\left(\frac{1/2}{2}-\frac{1}{3}+\frac{1/2}{4}\right)+\left(\frac{1/2}{3}-\frac{1}{4}+\frac{1/2}{5}\right)+\left(\frac{1/2}{4}-\frac{1}{5}+\frac{1/2}{6}\right)+\ldots+\left(\frac{1/2}{n-1}-\frac{1}{n}+\frac{1/2}{n+1}\right)+\left(\frac{1/2}{n}-\frac{1}{n+1}+\frac{2}{n+2}\right) \\
&=\left(\frac{1}{2}-\frac{1}{2}+\frac{1}{3}\right)+\left(\frac{1}{4}-\frac{1}{3}+\frac{1}{4}\right)+\left(-\frac{1}{4}+\frac{1}{5}\right)+\left(-\frac{1}{5}+\frac{1}{6}\right)+\ldots+\left(\frac{1}{2\left(n+1\right)}\right)+\left(-\frac{1}{n+1}+\frac{1}{2\left(n+2\right)}\right)=\frac{1}{4}+\frac{1}{2\left(n+1\right)}-\frac{1}{n+1}+\frac{1}{2\left(n+2\right)}
\end{aligned}
$$
